---
grade: 9
field: geometry
difficulty: 9
source: "<–Ω–∞—Ç–ø—Ä–µ–≤–∞—Ä / —Å–ø–∏—Å–∞–Ω–∏–µ / –≥–æ–¥–∏–Ω–∞>"
problem_id: geom_9_2015_iso_angle
language_original: <mk | en | sr | hr | ...>
translated: false

# 
tags:
  - geometry
  - trigonometry
  - isosceles_triangle
  - angle_bisector
related_skills:
  - trigonometric_identities
  - solving_equations
---

# Problem
Determine the angles of an isosceles triangle $ABC$, where the altitude to the base is half the length of the angle bisector of one of the base angles.

![Problem Visualization](media/geom_9_2015_iso_angle.mp4)

# Solution
Let the triangle be $ABC$ with $AC=BC$. Let $\alpha$ be the base angle $\angle A = \angle B$, and $\gamma$ be the vertex angle $\angle C$.
Let $h_c$ be the altitude to the base $AB$, and $l_\alpha$ be the angle bisector of $\angle A$.
We are given $l_\alpha = 2 h_c$.

In the right-angled triangle $ADC$ (where $D$ is the midpoint of $AB$), we have:
$$h_c = AC \sin \alpha$$

The length of the angle bisector $l_\alpha$ is given by the formula:
$$l_\alpha = \frac{2 AC \cdot AB \cos(\alpha/2)}{AC + AB}$$
Since $AB = 2 AC \cos \alpha$, we can substitute:
$$l_\alpha = \frac{2 AC \cdot (2 AC \cos \alpha) \cos(\alpha/2)}{AC + 2 AC \cos \alpha} = \frac{4 AC^2 \cos \alpha \cos(\alpha/2)}{AC(1 + 2 \cos \alpha)} = \frac{4 AC \cos \alpha \cos(\alpha/2)}{1 + 2 \cos \alpha}$$

We are given $l_\alpha = 2 h_c$. Substituting $h_c = AC \sin \alpha$:
$$\frac{4 AC \cos \alpha \cos(\alpha/2)}{1 + 2 \cos \alpha} = 2 AC \sin \alpha$$

Dividing by $2 AC$ (since $AC \neq 0$):
$$\frac{2 \cos \alpha \cos(\alpha/2)}{1 + 2 \cos \alpha} = \sin \alpha$$
$$2 \cos \alpha \cos(\alpha/2) = \sin \alpha (1 + 2 \cos \alpha)$$

Using $\sin \alpha = 2 \sin(\alpha/2) \cos(\alpha/2)$:
$$2 \cos \alpha \cos(\alpha/2) = 2 \sin(\alpha/2) \cos(\alpha/2) (1 + 2 \cos \alpha)$$

Since $\alpha < 90^\circ$, $\cos(\alpha/2) \neq 0$, so we can divide by $2 \cos(\alpha/2)$:
$$\cos \alpha = \sin(\alpha/2) (1 + 2 \cos \alpha)$$
$$\cos \alpha = \sin(\alpha/2) + 2 \sin(\alpha/2) \cos \alpha$$
$$\cos \alpha (1 - 2 \sin(\alpha/2)) = \sin(\alpha/2)$$

Let $x = \sin(\alpha/2)$. Then $\cos \alpha = 1 - 2 \sin^2(\alpha/2) = 1 - 2x^2$.
$$(1 - 2x^2)(1 - 2x) = x$$
$$1 - 2x - 2x^2 + 4x^3 = x$$
$$4x^3 - 2x^2 - 3x + 1 = 0$$

We check for rational roots. $x=1$ is a root since $4-2-3+1=0$.
Dividing by $(x-1)$:
$$(x-1)(4x^2 + 2x - 1) = 0$$

Since $x = \sin(\alpha/2) < 1$ (as $\alpha < 180^\circ$), we solve $4x^2 + 2x - 1 = 0$:
$$x = \frac{-2 \pm \sqrt{4 - 4(4)(-1)}}{8} = \frac{-2 \pm \sqrt{20}}{8} = \frac{-1 \pm \sqrt{5}}{4}$$

Since $x > 0$, we take the positive root:
$$x = \frac{\sqrt{5}-1}{4}$$

This value corresponds to $\sin(18^\circ)$.
So $\alpha/2 = 18^\circ \implies \alpha = 36^\circ$.

The angles of the triangle are:
$$\angle A = \angle B = 36^\circ$$
$$\angle C = 180^\circ - 2(36^\circ) = 108^\circ$$

The angles are $36^\circ, 36^\circ, 108^\circ$.

![Isosceles Angle](images/geom_9_2015_iso_angle.png)

## üí° –†–µ—à–µ–Ω–∏–µ

–ù–µ–∫–∞ –∞–≥–ª–∏—Ç–µ –ø—Ä–∏ –æ—Å–Ω–æ–≤–∞—Ç–∞ —Å–µ $\alpha$, –∞ –∞–≥–æ–ª–æ—Ç –ø—Ä–∏ –≤—Ä–≤–æ—Ç $\gamma$.
–í–∏—Å–∏–Ω–∞—Ç–∞ –∫–æ–Ω –æ—Å–Ω–æ–≤–∞—Ç–∞ –µ $h_c = a \sin \alpha$, –∫–∞–¥–µ $a$ –µ –¥–æ–ª–∂–∏–Ω–∞—Ç–∞ –Ω–∞ –∫—Ä–∞–∫–æ—Ç.
–°–∏–º–µ—Ç—Ä–∞–ª–∞—Ç–∞ –Ω–∞ –∞–≥–æ–ª–æ—Ç $\alpha$ –µ $l_a$.
–í–æ —Ç—Ä–∏–∞–≥–æ–ª–Ω–∏–∫–æ—Ç $ABD$ (–∫–∞–¥–µ $AD$ –µ —Å–∏–º–µ—Ç—Ä–∞–ª–∞), –∞–≥–ª–∏—Ç–µ —Å–µ $\alpha/2$, $\beta = \alpha$, –∏ $\angle ADB = 180^\circ - 1.5\alpha$.
–°–ø–æ—Ä–µ–¥ —Å–∏–Ω—É—Å–Ω–∞—Ç–∞ —Ç–µ–æ—Ä–µ–º–∞ –∑–∞ $\triangle ABD$:
$$ \frac{l_a}{\sin \beta} = \frac{c}{\sin(180^\circ - 1.5\alpha)} $$
$$ \frac{l_a}{\sin \alpha} = \frac{c}{\sin(1.5\alpha)} \implies l_a = \frac{c \sin \alpha}{\sin(1.5\alpha)} $$
–ò—Å—Ç–æ —Ç–∞–∫–∞, –≤–æ –ø—Ä–∞–≤–æ–∞–≥–æ–ª–Ω–∏–æ—Ç —Ç—Ä–∏–∞–≥–æ–ª–Ω–∏–∫ $AMC$ (–∫–∞–¥–µ $M$ –µ —Å—Ä–µ–¥–∏–Ω–∞ –Ω–∞ $AB$), –∏–º–∞–º–µ:
$$ \tan \alpha = \frac{h_c}{c/2} \implies h_c = \frac{c}{2} \tan \alpha $$
–î–∞–¥–µ–Ω–æ –µ –¥–µ–∫–∞ $h_c = \frac{l_a}{2}$. –ó–∞–º–µ–Ω—É–≤–∞–º–µ:
$$ \frac{c}{2} \tan \alpha = \frac{1}{2} \frac{c \sin \alpha}{\sin(1.5\alpha)} $$
$$ \tan \alpha = \frac{\sin \alpha}{\sin(1.5\alpha)} $$
$$ \frac{\sin \alpha}{\cos \alpha} = \frac{\sin \alpha}{\sin(1.5\alpha)} $$
–ë–∏–¥–µ—ò—ú–∏ $\alpha$ –µ –∞–≥–æ–ª –≤–æ —Ç—Ä–∏–∞–≥–æ–ª–Ω–∏–∫, $\sin \alpha \neq 0$, –ø–∞ –º–æ–∂–µ–º–µ –¥–∞ —Å–∫—Ä–∞—Ç–∏–º–µ:
$$ \frac{1}{\cos \alpha} = \frac{1}{\sin(1.5\alpha)} \implies \cos \alpha = \sin(1.5\alpha) $$
–ö–æ—Ä–∏—Å—Ç–∏–º–µ –∏–¥–µ–Ω—Ç–∏—Ç–µ—Ç $\cos \alpha = \sin(90^\circ - \alpha)$:
$$ \sin(90^\circ - \alpha) = \sin(1.5\alpha) $$
–†–µ—à–µ–Ω–∏—ò–∞—Ç–∞ —Å–µ:
1. $90^\circ - \alpha = 1.5\alpha \implies 2.5\alpha = 90^\circ \implies \alpha = 36^\circ$.
2. $90^\circ - \alpha = 180^\circ - 1.5\alpha \implies 0.5\alpha = 90^\circ \implies \alpha = 180^\circ$ (–Ω–µ–≤–æ–∑–º–æ–∂–Ω–æ).

–ó–Ω–∞—á–∏, –∞–≥–ª–∏—Ç–µ –ø—Ä–∏ –æ—Å–Ω–æ–≤–∞—Ç–∞ —Å–µ $\alpha = 36^\circ$.
–ê–≥–æ–ª–æ—Ç –ø—Ä–∏ –≤—Ä–≤–æ—Ç –µ $\gamma = 180^\circ - 2\alpha = 180^\circ - 72^\circ = 108^\circ$.
–ê–≥–ª–∏—Ç–µ –Ω–∞ —Ç—Ä–∏–∞–≥–æ–ª–Ω–∏–∫–æ—Ç —Å–µ $36^\circ, 36^\circ, 108^\circ$. 
5. $2\alpha + \frac{\alpha}{2} = 90^\circ \implies 5\alpha = 180^\circ \implies \alpha = 36^\circ$. 
6. –ê–≥–ª–∏—Ç–µ —Å–µ $36^\circ, 36^\circ, 108^\circ$.

## ‚ö†Ô∏è –ê–Ω–∞–ª–∏—Ç–∏—á–∫–∏ –ø—Ä–∏—Å—Ç–∞–ø (—Å–∞–º–æ –∞–∫–æ –µ –Ω–µ–∏–∑–±–µ–∂–µ–Ω)
<–ê–∫–æ –º–æ—Ä–∞ –¥–∞ —Å–µ –∫–æ—Ä–∏—Å—Ç–∞—Ç –∫–æ–æ—Ä–¥–∏–Ω–∞—Ç–∏, –æ–±—ò–∞—Å–Ω–∏ –∑–æ—à—Ç–æ —Å–∏–Ω—Ç–µ—Ç–∏—á–∫–∏–æ—Ç –ø–∞—Ç –µ –ø—Ä–µ—Ç–µ–∂–æ–∫.>

## üèÅ –ó–∞–∫–ª—É—á–æ–∫
–í–∏–¥–µ—Ç–µ –≥–æ —Ä–µ—à–µ–Ω–∏–µ—Ç–æ –ø–æ–≥–æ—Ä–µ.